\section{Kernels I}

Consider $\mathbf{x}$, $\mathbf{y} \in \mathbb{R}^d$, $d \in \mathbb{N}$. 
Explain in detail why each of the following functions is or is not a valid 
kernel:\bigskip

\Problem{$K(x,y)=x^Ty+(x^Ty)^2$}\medskip

\Solution{
First of all, expanding the term raised to power, it is obtained the expression 
$K(x,y)=x^Ty+(x^Ty)(x^Ty)$. $K(x,y)=x^Ty$ is a linear kernel, so it is valid. 
Using this knowledge,
\begin{equation*}
K(x,y)=x^Ty+(x^Ty)(x^Ty)=K_1(x, y)+K_2(x,y)\times K_3(x,y) \mbox{.}
\end{equation*}
Since the sum and the multiplication of two valid kernels produce a valid 
kernel, taking advantage of this two rules: \begin{itemize}
	\item $K(x,y)=K_1(x,y)+K_2(x,y)$
	\item $K(x,y)=K_1(x,y)\times K_2(x,y)$,
\end{itemize} 
so it is proved that the following is a valid kernel 
\begin{align*}
	K(x,y) & =x^Ty+(x^Ty)(x^Ty)=K_1(x^T, y)+K_2(x^T,y)\times K_3(x^T,y)= \\
	& = K_1(x^T,y)+K_4(x^T,y)=K_5(x^T,y)=x^Ty
\end{align*}
}

\Problem{$K(x,y)=x^2e^{-y}$, $d=1$}\medskip

\Solution{
%FIXME
As in the previous exercise, the term raised to power can be write as 
$x^2=x\times x$. In this case $K(x,x)=x x$ is a linear kernel, so it is valid. 
But $e^{-y}=e^{-1}e^y$ it is not symmetric, so we cannot prove that 
$K(x,y)=x^2e^{-y}$ is 
a valid kernel.
}\vspace{.5cm}

\Problem{$K(x,y)=ck_1(x,y)+k_2(x,y)$, where $k_1(x,y)$, $k_2(x,y)$ are 
	valid kernels in $\mathbb{R}^d$}\medskip

\Solution{
It is already known that $k_1(x,y)$ and $k_2(x,y)$ are valid kernels.
Since multiplying a valid kernel for a constant it remains a valid kernel, and 
since the sum of two valid kernels produce a valid kernel, taking advantage of 
this two rules: \begin{itemize}
	\item $K(x,y)=c \times K_1(x,y) \quad \mathrm{ with } \: c > 0 \: \mathrm{ 
	constant }$
	\item $K(x,y)=K_1(x,y)+K_2(x,y)$,
\end{itemize} 
so it is proved that, only if the constant is positive, the following is a 
valid kernel 
\begin{equation*}
K(x,y)=c \, K_1(x,y) + K_2(x,y)= K_3(x,y) + K_2(x,y)= K_4(x,y)
\end{equation*}
}
